viper-total-heaps/TotalSemanticsCoreHelper.thy
@@ -259,4 +259,14 @@ subsubsection \<open>Unfold\<close>
 
 (* inductive_cases UnfoldRel_case: "unfold_rel ctxt pred_id vs q \<phi> \<phi>'" *)
 
+
+subsection \<open>Ported from TotalExpressions.thy\<close>
+
+\<comment> \<open>Do we need \<^term>\<open>StateCons\<close> here?\<close>
+
+definition assertion_framing_state :: "'a total_context \<Rightarrow> ('a full_total_state \<Rightarrow> bool) \<Rightarrow> assertion \<Rightarrow> 'a full_total_state \<Rightarrow> bool"
+  where
+    "assertion_framing_state ctxt StateCons A \<omega> \<equiv>
+      \<forall> res. red_inhale ctxt A \<omega> res \<longrightarrow> res \<noteq> RFailure"
+
 end
